theories/SepBase.v
@@ -48,7 +48,7 @@ Definition heap : Type := (state)%type.
 Definition heap_affine (h:heap) := True.
 
 (** For uniformity with other instantiations of the Separation Logic
-  functor, we introduce local names for operations and lemmas on heaps. *)
+  functor, we introduce mklocal names for operations and lemmas on heaps. *)
 
 Definition heap_empty : heap := fmap_empty.
 
@@ -540,12 +540,12 @@ End HoarePrimitives.
 Definition triple (t:trm) (H:hprop) (Q:val->hprop) :=
   forall H', hoare t (H \* H') (Q \*+ H' \*+ \GC).
 
-(** SL triples satisfy [is_local], in the sense of SepFunctor *)
+(** SL triples satisfy [local], in the sense of SepFunctor *)
 
-Lemma is_local_triple : forall t,
-  is_local (triple t).
+Lemma local_triple : forall t,
+  local (triple t).
 Proof using.
-  intros. applys is_local_intro. intros H Q M H'. 
+  intros. applys local_intro. intros H Q M H'. 
   applys hoare_named_heap. intros h (h1&h2&N1&N2&N3&N4).
   lets (H1&H2&Q1&M0): (rm M) (rm N1).
   rewrite <- hstar_assoc, hstar_comm, hstar_hpure in M0.
@@ -555,7 +555,7 @@ Proof using.
   { intros x. hchanges (M2 x). }
 Qed.
 
-Hint Resolve is_local_triple.
+Hint Resolve local_triple.
 
 (** Lemma to introduce hoare instances for establishing triples,
     integrating the consequence rule. *)
@@ -585,24 +585,24 @@ Lemma triple_conseq : forall t H' Q' H Q,
   H ==> H' ->
   Q' ===> Q ->
   triple t H Q.
-Proof using. intros. applys* is_local_conseq. Qed.
+Proof using. intros. applys* local_conseq. Qed.
 
 Lemma triple_frame : forall t H Q H',
   triple t H Q ->
   triple t (H \* H') (Q \*+ H').
-Proof using. intros. applys* is_local_frame. Qed.
+Proof using. intros. applys* local_frame. Qed.
 
 Lemma triple_ramified_frame : forall H1 Q1 t H Q,
   triple t H1 Q1 ->
   H ==> H1 \* (Q1 \--* Q) ->
   triple t H Q.
-Proof using. intros. applys* is_local_ramified_frame. Qed.
+Proof using. intros. applys* local_ramified_frame. Qed.
 
 Lemma triple_ramified_frame_hgc : forall H1 Q1 t H Q,
   triple t H1 Q1 ->
   H ==> H1 \* (Q1 \--* (Q \*+ \GC)) ->
   triple t H Q.
-Proof using. intros. applys* is_local_ramified_frame_hgc. Qed.
+Proof using. intros. applys* local_ramified_frame_hgc. Qed.
 
 Lemma triple_ramified_frame_htop : forall H1 Q1 t H Q,
   triple t H1 Q1 ->
@@ -613,12 +613,12 @@ Proof using. introv M1 W. rewrite <- hgc_eq_htop in W. applys* triple_ramified_f
 Lemma triple_hgc_pre : forall t H Q,
   triple t H Q ->
   triple t (H \* \GC) Q.
-Proof using. intros. applys* is_local_hgc_pre. Qed.
+Proof using. intros. applys* local_hgc_pre. Qed.
 
 Lemma triple_hgc_post : forall t H Q,
   triple t H (Q \*+ \GC) ->
   triple t H Q.
-Proof using. intros. applys* is_local_hgc_post. Qed.
+Proof using. intros. applys* local_hgc_post. Qed.
 
 Lemma triple_htop_pre : forall t H Q,
   triple t H Q ->
@@ -650,58 +650,58 @@ Qed.
 Lemma triple_hexists : forall t (A:Type) (J:A->hprop) Q,
   (forall x, triple t (J x) Q) ->
   triple t (hexists J) Q.
-Proof using. intros. applys* is_local_hexists. Qed.
+Proof using. intros. applys* local_hexists. Qed.
 
 Lemma triple_hforall : forall A (x:A) t (J:A->hprop) Q,
   triple t (J x) Q ->
   triple t (hforall J) Q.
-Proof using. intros. applys* is_local_hforall. Qed.
+Proof using. intros. applys* local_hforall. Qed.
 
 Lemma triple_hforall_exists : forall t A (J:A->hprop) Q, (* TODO: needed?*)
   (exists x, triple t (J x) Q) ->
   triple t (hforall J) Q.
-Proof using. intros. applys* is_local_hforall_exists. Qed.
+Proof using. intros. applys* local_hforall_exists. Qed.
 
 Lemma triple_hpure : forall t (P:Prop) H Q,
   (P -> triple t H Q) ->
   triple t (\[P] \* H) Q.
-Proof using. intros. applys* is_local_hpure. Qed.
+Proof using. intros. applys* local_hpure. Qed.
 
 Lemma triple_hwand_hpure_l : forall t (P:Prop) H Q,
   P ->
   triple t H Q ->
   triple t (\[P] \-* H) Q.
-Proof using. intros. applys* is_local_hwand_hpure_l. Qed.
+Proof using. intros. applys* local_hwand_hpure_l. Qed.
 
 Lemma triple_hor : forall t H1 H2 Q,
   triple t H1 Q ->
   triple t H2 Q ->
   triple t (hor H1 H2) Q.
-Proof using. intros. applys* is_local_hor. Qed.
+Proof using. intros. applys* local_hor. Qed.
 
 Lemma triple_hand_l : forall t H1 H2 Q,
   triple t H1 Q ->
   triple t (hand H1 H2) Q.
-Proof using. intros. applys* is_local_hand_l. Qed.
+Proof using. intros. applys* local_hand_l. Qed.
 
 Lemma triple_hand_r : forall t H1 H2 Q,
   triple t H2 Q ->
   triple t (hand H1 H2) Q.
-Proof using. intros. applys* is_local_hand_r. Qed.
+Proof using. intros. applys* local_hand_r. Qed.
 
 Lemma triple_conseq_frame : forall H2 H1 Q1 t H Q,
   triple t H1 Q1 ->
   H ==> H1 \* H2 ->
   Q1 \*+ H2 ===> Q ->
   triple t H Q.
-Proof using. intros. applys* is_local_conseq_frame. Qed.
+Proof using. intros. applys* local_conseq_frame. Qed.
 
 Lemma triple_conseq_frame_hgc : forall H2 H1 Q1 t H Q,
   triple t H1 Q1 ->
   H ==> H1 \* H2 ->
   Q1 \*+ H2 ===> Q \*+ \GC ->
   triple t H Q.
-Proof using. intros. applys* is_local_conseq_frame_hgc. Qed.
+Proof using. intros. applys* local_conseq_frame_hgc. Qed.
 
 
 (* ---------------------------------------------------------------------- *)
