theories/SepCredits.v
@@ -722,12 +722,12 @@ Proof using.
    math. }
 Qed.
 
-(** Triple satisfy the [is_local] predicate *)
+(** Triple satisfy the [local] predicate *)
 
-Lemma is_local_triple : forall t,
-  is_local (triple t).
+Lemma local_triple : forall t,
+  local (triple t).
 Proof using.
-  intros. applys is_local_intro. intros H Q M H'. 
+  intros. applys local_intro. intros H Q M H'. 
   intros h (h1&h2&N1&N2&N3&N4). hnf in M.
   lets (H1&H2&Q1&R): M N1.
   rewrite <- hstar_assoc, hstar_comm, hstar_hpure in R.
@@ -739,7 +739,7 @@ Proof using.
   hchange (R2 v). hsimpl.
 Qed.
 
-Hint Resolve is_local_triple.
+Hint Resolve local_triple.
 
 
 (* ---------------------------------------------------------------------- *)
@@ -757,71 +757,71 @@ Lemma triple_conseq : forall t H' Q' H Q,
   H ==> H' ->
   Q' ===> Q ->
   triple t H Q.
-Proof using. intros. applys* is_local_conseq. Qed.
+Proof using. intros. applys* local_conseq. Qed.
 
 Lemma triple_frame : forall t H Q H',
   triple t H Q ->
   triple t (H \* H') (Q \*+ H').
-Proof using. intros. applys* is_local_frame. Qed.
+Proof using. intros. applys* local_frame. Qed.
 
 Lemma triple_hgc_pre : forall t H Q,
   triple t H Q ->
   triple t (H \* \GC) Q.
-Proof using. intros. applys* is_local_hgc_pre. Qed.
+Proof using. intros. applys* local_hgc_pre. Qed.
 
 Lemma triple_hgc_post : forall t H Q,
   triple t H (Q \*+ \GC) ->
   triple t H Q.
-Proof using. intros. applys* is_local_hgc_post. Qed.
+Proof using. intros. applys* local_hgc_post. Qed.
 
 Lemma triple_hexists : forall t (A:Type) (J:A->hprop) Q,
   (forall x, triple t (J x) Q) ->
   triple t (hexists J) Q.
-Proof using. intros. applys* is_local_hexists. Qed.
+Proof using. intros. applys* local_hexists. Qed.
 
 Lemma triple_hforall : forall A (x:A) t (J:A->hprop) Q,
   triple t (J x) Q ->
   triple t (hforall J) Q.
-Proof using. intros. applys* is_local_hforall. Qed.
+Proof using. intros. applys* local_hforall. Qed.
 
 Lemma triple_hforall_exists : forall t A (J:A->hprop) Q, (* TODO: needed?*)
   (exists x, triple t (J x) Q) ->
   triple t (hforall J) Q.
-Proof using. intros. applys* is_local_hforall_exists. Qed.
+Proof using. intros. applys* local_hforall_exists. Qed.
 
 Lemma triple_hpure : forall t (P:Prop) H Q,
   (P -> triple t H Q) ->
   triple t (\[P] \* H) Q.
-Proof using. intros. applys* is_local_hpure. Qed.
+Proof using. intros. applys* local_hpure. Qed.
 
 Lemma triple_hwand_hpure_l : forall t (P:Prop) H Q,
   P ->
   triple t H Q ->
   triple t (\[P] \-* H) Q.
-Proof using. intros. applys* is_local_hwand_hpure_l. Qed.
+Proof using. intros. applys* local_hwand_hpure_l. Qed.
 
 Lemma triple_hor : forall t H1 H2 Q,
   triple t H1 Q ->
   triple t H2 Q ->
   triple t (hor H1 H2) Q.
-Proof using. intros. applys* is_local_hor. Qed.
+Proof using. intros. applys* local_hor. Qed.
 
 Lemma triple_hand_l : forall t H1 H2 Q,
   triple t H1 Q ->
   triple t (hand H1 H2) Q.
-Proof using. intros. applys* is_local_hand_l. Qed.
+Proof using. intros. applys* local_hand_l. Qed.
 
 Lemma triple_hand_r : forall t H1 H2 Q,
   triple t H2 Q ->
   triple t (hand H1 H2) Q.
-Proof using. intros. applys* is_local_hand_r. Qed.
+Proof using. intros. applys* local_hand_r. Qed.
 
 Lemma triple_conseq_frame_hgc : forall H2 H1 Q1 t H Q,
   triple t H1 Q1 ->
   H ==> H1 \* H2 ->
   Q1 \*+ H2 ===> Q \*+ \GC ->
   triple t H Q.
-Proof using. intros. applys* is_local_conseq_frame_hgc. Qed.
+Proof using. intros. applys* local_conseq_frame_hgc. Qed.
 
 (* TODO: move to SepFunctor? *)
 
